fixes

template-coq/theories/Inductives.v
@@ -1,5 +1,7 @@
-From MetaCoq.Template Require Import utils BasicAst.
-From MetaCoq.Template Require Import Universes Environment Declarations.
+
+From MetaCoq.Checker Require Import Checker. 
+From MetaCoq.Template Require Import utils BasicAst Ast AstUtils.
+From MetaCoq.Template Require Import Universes Environment Declarations Reflect. 
 From MetaCoq.Template.utils Require Import RTree. 
 
 
@@ -31,37 +33,81 @@ Definition except {X Y: Type} (def : Y) (x : option X) : X + Y :=
   | Some x => inl x
   | None => inr def
   end.
+Definition raise {X Y : Type} (def : Y) : X + Y := inr def. 
 Notation "'exc' A" := ((A + string)%type) (at level 100). 
 
-Notation "f '$' a" := (f (a)) (at level 99). 
+Notation "f '$' a" := (f (a)) (at level 99, only parsing). 
+
+
+Notation "a == b" := (eqb a b) (at level 90). 
+Notation "a != b" := (negb(a==b)) (at level 90).
+
+
+Class ExcUnwrap (Xl : Type -> Type) := exc_unwrap X : Xl (exc X) -> exc (Xl X).
+Arguments exc_unwrap {_ _ _}. 
+
+Fixpoint list_unwrap {X : Type} (l : list (exc X)) : exc (list X) := 
+  match l with 
+  | [] => ret []
+  | x :: l => 
+      x <- x ;;
+      l <- list_unwrap l;;
+      ret (x :: l)
+  end.
+Instance: ExcUnwrap list := @list_unwrap. 
 
 
 (** WIP : An implementation of the guardedness checker *)
 
-Module Guarded (T : Term) (D : DeclarationsSig T). 
-  Import T D. 
-
-  Definition mind_definition := mutual_inductive_body * one_inductive_body. 
+Implicit Types (Σ : global_env) (c : context). 
+Definition whd_all Σ c t := 
+  except "whd_all: out of fuel" $ reduce_opt RedFlags.default Σ c default_fuel t. 
 
 (* head-normalized constructor types so that their conclusion exposes the inductive type -- context contains the parameters *)
-(*TODO *)
-(*Definition ind_ctors_hnf (i : mind_specif) : list (context * term) := *)
-  (*let (mib, oib) := npars in*)
-  (*[]. *)
+(* TODO : similar to ind_user_lc, this might not reflect the actual Coq definition *)
+Definition ind_ctors_hnf (i : mind_specif) : exc (list (context * term)) := 
+  let (mib, oib) := i in
+  let npars := mib.(ind_npars) in 
+  let without_params := map (fun t => snd (decompose_prod_n t npars)) (ind_user_lc (mib, oib)) in 
+  let params := param_ctxt (mib, oib) in
+  hnfed <- exc_unwrap $ map (whd_all [] params) without_params;;
+  ret (map (fun t => (params, t)) hnfed).
 
 
-  
-  Definition lookup_mind_definition Σ (ind : inductive) := 
-    mib <- except "lookup_mind_definition: could not find inductive" $ 
-      lookup_env_mind Σ ind.(inductive_mind) ;;
-    ib <- except "lookup_mind_definition: invalid inductive index" $ 
-      nth_error mib.(ind_bodies) ind.(inductive_ind) ;;
-    ret (mib, ib).
+Definition lookup_env_mind Σ kn : option mutual_inductive_body := 
+  match lookup_env Σ kn with 
+  | Some (InductiveDecl ind) => Some ind
+  | _ => None
+  end.
+
+Definition lookup_mind_specif Σ (ind : inductive) : exc mind_specif := 
+  mib <- except "lookup_mind_specif: could not find inductive" $ 
+    lookup_env_mind Σ ind.(inductive_mind) ;;
+  ib <- except "lookup_mind_specif: invalid inductive index" $ 
+    nth_error mib.(ind_bodies) ind.(inductive_ind) ;;
+  ret (mib, ib).
 
 
-End Guarded.
+(* if c evaluates to an application (weak-head) and the LHS is an inductive, return it together with the RHS (list) *)
+Definition find_rectype Σ c t := 
+  t <- whd_all Σ c t;; 
+  let (t, l) := decompose_app t in 
+  match t with 
+  | tInd i u => ret ((i, u), l)
+  | _ => raise "find_rectype"
+  end. 
 
 
+(* the same, but only if the rectype is an inductive or record (bifinite) *)
+Definition find_inductive Σ c t := 
+  '((i, u), l) <- find_rectype Σ c t;;
+  '(mib, _) <- lookup_mind_specif Σ i;;
+  if mib.(ind_finite) != CoFinite then ret ((i, u), l) else raise "find_inductive: is cofinite".
 
-Import Environment.
-Check Environment.mutual_inductive_body.
+(* only if coinductive *)
+Definition find_coinductive Σ c t := 
+  '((i, u), l) <- find_rectype Σ c t;;
+  '(mib, _) <- lookup_mind_specif Σ i;;
+  if mib.(ind_finite) == CoFinite then ret ((i, u), l) else raise "find_coinductive: is not cofinite".
+
+
